QSemanticsBig.thy
@@ -1,0 +1,191 @@
+(* Title:     Quantum-Semantics/QSemantics.thy
+   Author:    David Sanan, Nanyang Technological University 
+   Copyright   2020
+   License:     BSD
+*)
+
+theory QSemanticsBig
+  imports QSyntax  
+begin           
+
+subsection \<open>Syntax\<close>
+
+text \<open>Semantics for quantum programs\<close>
+
+(* m = partial_state2.ptensor_mat (dims_heap \<vv>) (q \<sigma>) ((Q_domain \<vv>)-(q \<sigma>)) (M::complex mat) (1\<^sub>m (card ((Q_domain \<vv>) - (q \<sigma>))))*)
+(* abbreviation "tensor_vec \<equiv> partial_state2.ptensor_vec" *)
+
+definition
+  unit_vecl :: "nat \<Rightarrow> nat \<Rightarrow> complex list"
+  where "unit_vecl n i = list_of_vec (unit_vec n i)"
+
+definition matrix_sep :: "nat set \<Rightarrow> qstate \<Rightarrow> complex mat \<Rightarrow> qstate" 
+  where "matrix_sep sep_vars q M \<equiv>
+           let qs = snd q in
+           let var_d = QState_vars qs in 
+           let var_r = var_d - sep_vars in
+           let v = QState_vector qs in           
+           let m = partial_state2.ptensor_mat sep_vars var_r
+                                        (M::complex mat) (1\<^sub>m (2^(card var_r)))  in           
+             (fst q, QState (var_d, list_of_vec (m *\<^sub>v v)))
+        "
+
+definition measure_vars1::"nat \<Rightarrow>  nat set \<Rightarrow> qstate  \<Rightarrow> (real \<times> qstate)"
+  where "measure_vars1 k  sep_vars q \<equiv>
+   let qs = snd q in
+   let vars_dom = QState_vars qs in
+    let v =   QState_vector qs in
+    let vars= (vars_dom - sep_vars) in    
+    let mk = partial_state2.ptensor_mat  vars_dom vars (1\<^sub>k (2^(card vars_dom))) (1\<^sub>m (2^(card vars))) in
+    let qn' =  mk  *\<^sub>v v in 
+    let \<delta>k =  Re (((mat_adjoint (mat_of_rows (dim_vec v) [v]) *\<^sub>v qn') $ 0) div vec_norm qn') in    
+    let qnprod = list_of_vec (((sqrt \<delta>k)::complex) \<cdot>\<^sub>v qn') in
+       (\<delta>k, (fst q, QState (vars_dom, qnprod)))" 
+
+definition measure_vars::"nat \<Rightarrow>  nat set \<Rightarrow> qstate  \<Rightarrow> (real \<times> qstate)"
+  where "measure_vars k  sep_vars q \<equiv>
+   let qs = snd q in
+   let vars_dom = QState_vars qs in
+    let v =   QState_vector qs in
+    let vars= (vars_dom - sep_vars) in        
+    let mk = partial_state2.ptensor_mat  sep_vars vars (1\<^sub>k (2^(card sep_vars))) (1\<^sub>m (2^(card vars))) in
+    let v' =  mk  *\<^sub>v v in 
+    let \<delta>k =  Re ((vec_norm v')^2 div (vec_norm v)^2) in    
+    let qnprod = list_of_vec (((sqrt \<delta>k)::complex) \<cdot>\<^sub>v v') in
+       (\<delta>k, (fst q, QState (vars_dom, qnprod)))" 
+
+context vars
+begin
+
+
+inductive QExec::"('v, 's) com \<Rightarrow> 's XQState \<Rightarrow> 's XQState \<Rightarrow> bool" 
+  ("\<turnstile> \<langle>_,_\<rangle> \<Rightarrow> _"  [20,98,98] 89)  
+  where 
+  Skip : "\<turnstile>  \<langle>Skip, Normal \<sigma>\<rangle> \<Rightarrow> Normal \<sigma>" 
+\<comment>\<open>SMod  modifies the stack of non-qubits variables \<sigma> with f \<sigma>, where f is a 
+  function modifying the stack\<close>
+ | StackMod: "\<turnstile> \<langle>SMod f, Normal (\<delta>,\<sigma>,\<Q>)\<rangle> \<Rightarrow>  Normal (\<delta>,f \<sigma>,\<Q>)"
+
+\<comment>\<open>QMod modifies the set of qubits of the Quantum State given by q \<sigma> with the 
+  transformation matrix M, any qubit not included in q \<sigma> remains the same\<close>
+
+ | QMod:"(q (\<sigma>,\<vv>)) \<subseteq> (QState_vars \<qq>) \<Longrightarrow> 
+         \<qq>' = matrix_sep (q (\<sigma>,\<vv>)) (\<vv>,\<qq>) m \<Longrightarrow>
+         \<turnstile> \<langle>QMod M q, Normal (\<delta>,\<sigma>,(\<vv>,\<qq>))\<rangle> \<Rightarrow> Normal (\<delta>, \<sigma>, \<qq>')"
+
+\<comment>\<open>QMod fails if the set of qubits to be modified is not included in the quantum state\<close>
+ | QMod_F:"\<not> ((q (\<sigma>,\<vv>)) \<subseteq> (QState_vars \<qq>)) \<Longrightarrow>          
+          \<turnstile> \<langle>QMod M q, Normal (\<delta>,\<sigma>,(\<vv>,\<qq>))\<rangle> \<Rightarrow> Fault"
+
+\<comment>\<open>Alloc takes a normal variable "q" representing the variable where the index to the qubits is store
+   an function e from the state \<sigma> to a natural number representing the number of qubits to allocate
+  and an initialization value for the allocated qubits 
+
+
+  We will require that a program is well formed, meaning that the types are correct.
+  A call to Alloc is well formed if the type of q is a natural number\<close>
+
+ | Alloc:"q' \<notin> (dom_q_vars \<vv>) \<Longrightarrow> q'_addr \<in> new_q_addr e (\<delta>,\<sigma>,(\<vv>,\<qq>)) \<Longrightarrow> e \<sigma> \<noteq> 0 \<Longrightarrow> 
+          \<vv>' = \<vv>(q' := q'_addr)  \<Longrightarrow> length (v \<sigma>) = (e \<sigma>) \<Longrightarrow> \<sigma>' = set_value \<sigma> q (from_nat q') \<Longrightarrow>                    
+          \<turnstile> \<langle>Alloc q e v, Normal (\<delta>,\<sigma>,(\<vv>,\<qq>))\<rangle> \<Rightarrow> Normal (\<delta>, \<sigma>',(\<vv>',\<qq> + QState (q'_addr,(v \<sigma>)) ))"
+
+\<comment>\<open>Alloc will fail if the length of the initial value is not equal to the number of qubits allocated \<close>
+
+
+ | Alloc_F:"length (v \<sigma>) \<noteq> (e \<sigma>) \<or> e \<sigma> = 0 \<Longrightarrow>                    
+          \<turnstile> \<langle>Alloc q e v, Normal (\<delta>,\<sigma>,(\<vv>,\<qq>))\<rangle> \<Rightarrow> Fault"
+
+\<comment>\<open>the conditional, while, and seq statements follow the standard definitions\<close>
+
+ | CondTrue:"\<sigma>\<in>b \<Longrightarrow>  \<turnstile> \<langle>c1, Normal (\<delta>,\<sigma>,\<Q>)\<rangle> \<Rightarrow> \<sigma>' \<Longrightarrow> \<turnstile> \<langle>IF b c1 c2, Normal  (\<delta>,\<sigma>,\<Q>)\<rangle> \<Rightarrow> \<sigma>'"
+
+| CondFalse:"\<sigma>\<notin>b  \<Longrightarrow>  \<turnstile> \<langle>c2, Normal (\<delta>,\<sigma>,\<Q>)\<rangle> \<Rightarrow> \<sigma>' \<Longrightarrow> 
+           \<turnstile> \<langle>IF b c1 c2, Normal (\<delta>,\<sigma>,\<Q>)\<rangle> \<Rightarrow> \<sigma>'"
+
+ | WhileTrue: "\<sigma>\<in>b \<Longrightarrow> \<turnstile> \<langle>c, Normal (\<delta>,\<sigma>,\<Q>)\<rangle> \<Rightarrow> \<sigma>' \<Longrightarrow> \<turnstile> \<langle>While b c,\<sigma>'\<rangle> \<Rightarrow>  \<sigma>'' \<Longrightarrow>
+                \<turnstile> \<langle>While b c,Normal (\<delta>,\<sigma>,\<Q>)\<rangle> \<Rightarrow> \<sigma>''"
+
+ | WhileFalse: "\<sigma>\<notin>b \<Longrightarrow> 
+                 \<turnstile> \<langle>While b c,Normal  (\<delta>,\<sigma>,\<Q>)\<rangle> \<Rightarrow> Normal  (\<delta>,\<sigma>,\<Q>)"
+
+ | Seq:"\<lbrakk>\<turnstile> \<langle>C1, Normal \<sigma>\<rangle> \<Rightarrow> \<sigma>'; \<turnstile> \<langle>C2, \<sigma>'\<rangle> \<Rightarrow> \<sigma>'' \<rbrakk> \<Longrightarrow> \<turnstile> \<langle>Seq C1 C2, Normal \<sigma>\<rangle> \<Rightarrow> \<sigma>''"
+
+
+\<comment>\<open>Dispose takes an expression from the stack to a natural number and removes those qubits
+  from the quantum state if they are not entangled with the rest of qubits in the current
+  Quantum state. The entanglement condition is that it is possible to find a vector \<qq>1 such that
+  \<qq> =  \<qq>' +  \<qq>''\<close>
+
+ | Dispose: "\<vv> (q \<sigma>) \<noteq> {} \<Longrightarrow> \<vv>' = \<vv>((q \<sigma>):={}) \<Longrightarrow> \<qq>' ## \<qq>''  \<Longrightarrow> 
+            \<vv> (q \<sigma>) = QState_vars \<qq>'' \<Longrightarrow> \<qq> =   \<qq>' +  \<qq>'' \<Longrightarrow> 
+            n = vec_norm (QState_vector \<qq>'') \<Longrightarrow>                       
+             \<turnstile> \<langle>Dispose q, Normal (\<delta>,\<sigma>,(\<vv>,\<qq>))\<rangle> \<Rightarrow> Normal (\<delta>,\<sigma>,(\<vv>',n \<cdot>\<^sub>q \<qq>'))"                                  
+
+\<comment>\<open>Dispose dispose will fail if it is not possible to find such states \<qq>',  \<qq>''\<close>
+
+
+ | Dispose_F: "\<nexists>\<qq>' \<qq>''. \<vv> (q \<sigma>) \<noteq> {} \<and> \<vv> (q \<sigma>) = QState_vars \<qq>'' \<and> 
+               \<qq> =   \<qq>' +  \<qq>'' \<and> \<qq>' ## \<qq>'' \<Longrightarrow>
+               \<turnstile> \<langle>Dispose q, Normal (\<delta>,\<sigma>,(\<vv>,\<qq>))\<rangle> \<Rightarrow> Fault"
+
+\<comment>\<open>Measure measures the value of the set of qubits given by q \<sigma> and it stores the result in 
+  the stack variable v. Similar to allocate, we will require that the construct is well formed
+ and that the type of v is a real number\<close>
+
+ | Measure: "q (\<sigma>,\<vv>) = (QState_vars \<qq>1) \<Longrightarrow> k \<in> {0.. 2^(card (q (\<sigma>,\<vv>)))} \<Longrightarrow>
+            (\<delta>k, (\<vv>',\<qq>')) = measure_vars k (q (\<sigma>,\<vv>)) (\<vv>,\<qq>) \<Longrightarrow> \<qq> =   \<qq>1 +  \<qq>2 \<and> \<qq>1 ## \<qq>2 \<Longrightarrow>            
+            \<delta>k > 0 \<Longrightarrow> \<delta>' = \<delta> * \<delta>k \<Longrightarrow> \<sigma>' = set_value \<sigma> v (from_nat k) \<Longrightarrow>
+            \<turnstile> \<langle>Measure v q, Normal (\<delta>,\<sigma>,(\<vv>,\<qq>))\<rangle> \<Rightarrow> Normal (\<delta>',\<sigma>',(\<vv>',\<qq>'))" 
+
+\<comment>\<open>Since Measure access to the values of the qubits given by q \<sigma> as QMod, 
+  Measure will similarly fail if the set of qubits to be mesured does not
+  belong to the set of allocated qubits\<close>
+
+ | Measure_F: "\<not> (q (\<sigma>,\<vv>) \<subseteq> (QState_vars \<qq>)) \<Longrightarrow>  
+              \<turnstile> \<langle>Measure v q, Normal (\<delta>,\<sigma>,(\<vv>,\<qq>))\<rangle> \<Rightarrow> Fault" 
+
+| Fault_Prop:"\<turnstile> \<langle>C, Fault\<rangle> \<Rightarrow> Fault"
+
+
+
+inductive_cases QExec_elim_cases [cases set]:
+ "\<turnstile>\<langle>c,Fault\<rangle> \<Rightarrow>  t"  
+  "\<turnstile>\<langle>Skip,s\<rangle> \<Rightarrow>  t"
+  "\<turnstile>\<langle>SMod f,s\<rangle> \<Rightarrow>  t"
+  "\<turnstile>\<langle>QMod m q,s\<rangle> \<Rightarrow>  t"
+  "\<turnstile>\<langle>Seq c1 c2,s\<rangle> \<Rightarrow>  t"
+  "\<turnstile>\<langle>While b c,s\<rangle> \<Rightarrow>  t"
+  "\<turnstile>\<langle>IF b c1 c2,s\<rangle> \<Rightarrow>  t"
+  "\<turnstile>\<langle>Measure v q,s\<rangle> \<Rightarrow>  t"
+  "\<turnstile>\<langle>Alloc v q e,s\<rangle> \<Rightarrow>  t"
+  "\<turnstile>\<langle>Dispose q,s\<rangle> \<Rightarrow>  t"
+
+inductive_cases QExec_Normal_elim_cases [cases set]:
+ "\<turnstile>\<langle>c,Fault\<rangle> \<Rightarrow>  t"  
+  "\<turnstile>\<langle>Skip,Normal s\<rangle> \<Rightarrow>  t"
+  "\<turnstile>\<langle>SMod f,Normal s\<rangle> \<Rightarrow>  t"
+  "\<turnstile>\<langle>QMod m q,Normal s\<rangle> \<Rightarrow>  t"
+  "\<turnstile>\<langle>Seq c1 c2,Normal s\<rangle> \<Rightarrow>  t"
+  "\<turnstile>\<langle>While b c1,Normal s\<rangle> \<Rightarrow>  t"
+  "\<turnstile>\<langle>IF b c1 c2,Normal s\<rangle> \<Rightarrow>  t"
+  "\<turnstile>\<langle>Measure v q,Normal s\<rangle> \<Rightarrow>  t"
+  "\<turnstile>\<langle>Alloc v q e,Normal s\<rangle> \<Rightarrow>  t"
+  "\<turnstile>\<langle>Dispose q,Normal s\<rangle> \<Rightarrow>  t"
+
+primrec modify_locals :: "('v, 's) com  \<Rightarrow> 'v set" where 
+  "modify_locals  Skip = {}"
+| "modify_locals (SMod f) = {v. modify_v f v = True}"
+| "modify_locals (QMod _ _) = {}"
+| "modify_locals (IF b c1 c2) = modify_locals c1 \<union> modify_locals c2"
+| "modify_locals (While b c) = modify_locals c"
+| "modify_locals (Seq c1 c2) = modify_locals c1 \<union> modify_locals c2"
+| "modify_locals (Measure v e) = {v}"
+| "modify_locals (Alloc v e val) = {v}"
+| "modify_locals (Dispose e) = {}"
+
+thm QExec_Normal_elim_cases
+
+end 
+
+end
+
