vars.thy
@@ -13,34 +13,51 @@ subsection \<open>Syntax\<close>
 
 text \<open>Datatype for quantum programs\<close>
 
+class nat_abs=
+  fixes from_nat ::"nat \<Rightarrow> 'a"
+  fixes to_nat ::"'a \<Rightarrow> nat"
+  fixes subset_nat :: "'a set"
+
+  assumes "a \<in> subset_nat \<Longrightarrow> from_nat (to_nat a) = a "
+  assumes "to_nat (from_nat b) = b"
+
+class real_abs= nat_abs+
+  fixes from_real ::"real \<Rightarrow> 'a"
+  fixes to_real ::"'a \<Rightarrow> real"
+  fixes subset_real :: "'a set"
+
+  assumes "a \<in> subset_real \<Longrightarrow> from_real (to_real a) = a "
+  assumes "to_real (from_real b) = b"
+
 locale vars =  
   fixes variables :: "'v set"
-  fixes types :: "'v \<Rightarrow> 't"
-  fixes domain :: "'v \<Rightarrow> 'b set"
+  fixes v_domain :: "'v \<Rightarrow> ('b::nat_abs) set"
   fixes get_value :: "'s \<Rightarrow> 'v  \<Rightarrow> 'b"
-  fixes set_value ::"'s \<Rightarrow> 'v \<Rightarrow> 'b \<Rightarrow> 's"
-  fixes nat_to_typ ::"nat \<Rightarrow> 'b"
-  fixes typ_to_nat ::"'b \<Rightarrow> nat"
-  fixes conv::"('v \<Rightarrow> 'b) \<Rightarrow> 'v set \<Rightarrow> 's"
-                 
+  fixes set_value ::"'s \<Rightarrow> 'v \<Rightarrow> 'b \<Rightarrow> 's" 
+  fixes conv::"('v \<Rightarrow> 'b) \<Rightarrow> 'v set \<Rightarrow> 's"  
+
   assumes "finite variables"
-  assumes "v \<in> variables \<Longrightarrow> (get_value s v) \<in> domain v"
-  assumes eq_get_set:"x \<in> names \<Longrightarrow> get_value (set_value s v x) v = x"
-  assumes abs_elem: "s = conv ((get_value s)) variables"
+  assumes "v \<in> variables \<Longrightarrow> (get_value s v) \<in> v_domain v"
+  assumes eq_get_set:"v \<in> variables \<Longrightarrow> x \<in> (v_domain v) \<Longrightarrow> get_value (set_value s v x) v = x"
+  assumes abs_elem: "s = conv (get_value s) variables"
+  
 
 begin
 
 definition not_access_v::"('s \<Rightarrow> 'n) \<Rightarrow> 'v \<Rightarrow> bool"
 where "not_access_v f v \<equiv>     
-  \<forall>s f1 f2. f1\<in>domain v \<and> f2\<in> domain v \<longrightarrow>
+  \<forall>s f1 f2. f1 \<in> v_domain v \<and> f2 \<in> v_domain v \<longrightarrow>
     f (conv ((get_value s)(v:=f1)) variables) = 
     f (conv ((get_value s)(v:=f2)) variables)" 
 
 definition access_v::"('s \<Rightarrow> 'n) \<Rightarrow> 'v \<Rightarrow> bool"
 where "access_v f v \<equiv>     
-  \<exists>s f1 f2. f1\<in>domain v \<and> f2\<in> domain v \<and>
+  \<exists>s f1 f2. f1 \<in> v_domain v \<and> f2 \<in> v_domain v \<and>
     f (conv ((get_value s)(v:=f1)) variables) \<noteq> 
     f (conv ((get_value s)(v:=f2)) variables)"
+
+definition not_access_locals::"('s \<Rightarrow> 'n) \<Rightarrow> bool"
+where "not_access_locals f \<equiv> \<forall>v\<in>variables. not_access_v f v"
 
 lemma access_neg:"access_v f v = (\<not> (not_access_v f v))"
   unfolding access_v_def not_access_v_def by auto
@@ -55,6 +72,9 @@ lemma modify_neg:"modify_v f v =  ( \<not> (not_modify_v f v))"
   unfolding modify_v_def not_modify_v_def by auto
 
 end
+
+
+
 
 end
 
